Automatically hoisting kernel invocations

dist/Kuiper_BasicFloat.cu
@@ -4,9 +4,10 @@
 
 __global__
 
-static void kernel(float_t *r)
+static void __hoisted_0(float_t *gr, float_t *gr0)
 {
-  *r += (float_t)1.0f;
+  KRML_MAYBE_UNUSED_VAR(gr);
+  *gr0 += (float_t)1.0f;
 }
 
 float_t Kuiper_BasicFloat_main(void)
@@ -14,7 +15,7 @@ float_t Kuiper_BasicFloat_main(void)
   float_t r = (float_t)0.0f;
   float_t *gr = (float_t *)KPR_GPU_ALLOC((size_t)4U);
   MUST(cudaMemcpy(gr, &r, (size_t)4U, cudaMemcpyHostToDevice));
-  KPR_KCALL(kernel, (size_t)1U, (size_t)1U, (size_t)4U, (size_t)0U, gr);
+  KPR_KCALL(__hoisted_0, (size_t)1U, (size_t)1U, (size_t)4U, (size_t)0U, gr, gr);
   cudaDeviceSynchronize();
   MUST(cudaMemcpy(&r, gr, (size_t)4U, cudaMemcpyDeviceToHost));
   float_t v = r;
