dist/Kuiper_Example1.cu
@@ -4,9 +4,10 @@
 
 __global__
 
-static void kernel(uint64_t *r)
+static void __hoisted_0(uint64_t *gr, uint64_t *gr0)
 {
-  *r += 1ULL;
+  KRML_MAYBE_UNUSED_VAR(gr);
+  *gr0 += 1ULL;
 }
 
 uint64_t Kuiper_Example1_main(void)
@@ -14,7 +15,7 @@ uint64_t Kuiper_Example1_main(void)
   uint64_t r = 1ULL;
   uint64_t *gr = (uint64_t *)KPR_GPU_ALLOC((size_t)8U);
   MUST(cudaMemcpy(gr, &r, (size_t)8U, cudaMemcpyHostToDevice));
-  KPR_KCALL(kernel, (size_t)1U, (size_t)1U, (size_t)4U, (size_t)0U, gr);
+  KPR_KCALL(__hoisted_0, (size_t)1U, (size_t)1U, (size_t)4U, (size_t)0U, gr, gr);
   cudaDeviceSynchronize();
   MUST(cudaMemcpy(&r, gr, (size_t)8U, cudaMemcpyDeviceToHost));
   uint64_t v = r;
