dist/Kuiper_MatMul_Tiled_Inst.cu
@@ -5,23 +5,55 @@
 __global__
 
 static void
-k_u64_rrr(
+__hoisted_0(
   size_t bdim,
-  size_t rows,
-  size_t shared,
-  size_t cols,
+  size_t bdim0,
+  size_t mcols,
+  size_t mcols0,
+  size_t bdim1,
+  size_t bdim2,
+  size_t mshared,
+  size_t bdim3,
+  size_t mshared0,
+  size_t bdim4,
+  size_t bdim5,
   uint64_t *gA,
+  size_t bdim6,
+  size_t mcols1,
+  size_t bdim7,
+  size_t bdim8,
   uint64_t *gB,
+  size_t bdim9,
+  size_t bdim10,
+  size_t mcols2,
+  size_t bdim11,
+  size_t bdim12,
   uint64_t *gC
 )
 {
-  KRML_MAYBE_UNUSED_VAR(rows);
+  KRML_MAYBE_UNUSED_VAR(bdim);
+  KRML_MAYBE_UNUSED_VAR(bdim0);
+  KRML_MAYBE_UNUSED_VAR(mcols);
+  KRML_MAYBE_UNUSED_VAR(mcols0);
+  KRML_MAYBE_UNUSED_VAR(bdim1);
+  KRML_MAYBE_UNUSED_VAR(bdim2);
+  KRML_MAYBE_UNUSED_VAR(mshared);
+  KRML_MAYBE_UNUSED_VAR(bdim3);
+  KRML_MAYBE_UNUSED_VAR(bdim4);
+  KRML_MAYBE_UNUSED_VAR(bdim5);
+  KRML_MAYBE_UNUSED_VAR(bdim6);
+  KRML_MAYBE_UNUSED_VAR(mcols1);
+  KRML_MAYBE_UNUSED_VAR(bdim7);
+  KRML_MAYBE_UNUSED_VAR(bdim8);
+  KRML_MAYBE_UNUSED_VAR(bdim9);
+  KRML_MAYBE_UNUSED_VAR(bdim10);
+  KRML_MAYBE_UNUSED_VAR(bdim11);
   size_t bid = blockIdx_x();
   size_t tid = threadIdx_x();
-  size_t mrow = bid / cols;
-  size_t mcol = bid % cols;
-  size_t brow = tid / bdim;
-  size_t bcol = tid % bdim;
+  size_t mrow = bid / mcols2;
+  size_t mcol = bid % mcols2;
+  size_t brow = tid / bdim12;
+  size_t bcol = tid % bdim12;
   size_t bi = mrow;
   size_t bj = mcol;
   size_t i = brow;
@@ -29,14 +61,14 @@ k_u64_rrr(
   uint64_t sum = 0ULL;
   size_t bk = (size_t)0U;
   size_t k = (size_t)0U;
-  while (bk < shared)
+  while (bk < mshared0)
   {
     size_t vbk = bk;
     size_t vk = k;
     sum +=
-      gA[(mrow * bdim + brow) * (shared * bdim) + vbk * bdim + vk] *
-        gB[(vbk * bdim + vk) * (cols * bdim) + mcol * bdim + bcol];
-    if (vk == bdim - (size_t)1U)
+      gA[(mrow * bdim12 + brow) * (mshared0 * bdim12) + vbk * bdim12 + vk] *
+        gB[(vbk * bdim12 + vk) * (mcols2 * bdim12) + mcol * bdim12 + bcol];
+    if (vk == bdim12 - (size_t)1U)
     {
       k = (size_t)0U;
       bk = vbk + (size_t)1U;
@@ -44,7 +76,49 @@ k_u64_rrr(
     else
       k = vk + (size_t)1U;
   }
-  gC[(bi * bdim + i) * (cols * bdim) + bj * bdim + j] = sum;
+  gC[(bi * bdim12 + i) * (mcols2 * bdim12) + bj * bdim12 + j] = sum;
+}
+
+void
+Kuiper_MatMul_Tiled_Inst_matmul_gpu_u64_rrr(
+  size_t bdim,
+  size_t mrows,
+  size_t mshared,
+  size_t mcols,
+  uint64_t *gA,
+  uint64_t *gB,
+  uint64_t *gC
+)
+{
+  KPR_KCALL(__hoisted_0,
+    mrows * mcols,
+    bdim * bdim,
+    (size_t)4U,
+    (size_t)0U,
+    bdim,
+    bdim,
+    mcols,
+    mcols,
+    bdim,
+    bdim,
+    mshared,
+    bdim,
+    mshared,
+    bdim,
+    bdim,
+    gA,
+    bdim,
+    mcols,
+    bdim,
+    bdim,
+    gB,
+    bdim,
+    bdim,
+    mcols,
+    bdim,
+    bdim,
+    gC);
+  cudaDeviceSynchronize();
 }
 
 uint64_t
@@ -65,19 +139,7 @@ uint64_t
   uint64_t *gC = (uint64_t *)KPR_GPU_ALLOC((size_t)8U * (mrows * bdim * mcols * bdim));
   MUST(cudaMemcpy(gB, b, (size_t)8U * (mshared * bdim * (mcols * bdim)), cudaMemcpyHostToDevice));
   MUST(cudaMemcpy(gA, a, (size_t)8U * (mrows * bdim * (mshared * bdim)), cudaMemcpyHostToDevice));
-  KPR_KCALL(k_u64_rrr,
-    mrows * mcols,
-    bdim * bdim,
-    (size_t)4U,
-    (size_t)0U,
-    bdim,
-    mrows,
-    mshared,
-    mcols,
-    gA,
-    gB,
-    gC);
-  cudaDeviceSynchronize();
+  Kuiper_MatMul_Tiled_Inst_matmul_gpu_u64_rrr(bdim, mrows, mshared, mcols, gA, gB, gC);
   KRML_CHECK_SIZE(sizeof (uint64_t), rows * cols);
   uint64_t *c = (uint64_t *)KRML_HOST_CALLOC(rows * cols, sizeof (uint64_t));
   MUST(cudaMemcpy(c, gC, (size_t)8U * (mrows * bdim * (mcols * bdim)), cudaMemcpyDeviceToHost));
