src/lib/kuiper/Kuiper.Kernel.Nop.fsti
@@ -1,0 +1,130 @@
+module Kuiper.Kernel.Nop
+#lang-pulse
+
+open Kuiper.Common
+open Pulse.Lib.Core
+open FStar.Ghost
+open Kuiper.IntAliases
+open Kuiper.Array
+open Kuiper.Base
+module SZ = FStar.SizeT
+open Kuiper.ForEvery
+
+open Kuiper.Kernel.Base
+
+ghost
+fn nop_block_setup (#nblk #nthr : nat) (ar : gpu_array u32 0sz) (bid : natlt nblk)
+  requires
+    block_setup nthr ** (exists* v. gpu_pts_to_array ar v)
+  ensures
+    block_setup nthr ** (forall+ (i : natlt nthr). emp)
+{
+  drop_ (exists* v. gpu_pts_to_array ar v);
+  assume (forall+ (i : natlt nthr). emp); (* trivial to prove *)
+}
+
+ghost
+fn ghost_setup (#f:slprop) ()
+  requires f
+  ensures forall+ (ebid:natlt 1) (etid:natlt 1). f
+{
+  forevery_singleton_intro #(natlt 1) _;
+  forevery_singleton_intro #(natlt 1) _;
+}
+
+ghost
+fn ghost_teardown (#f:slprop) ()
+  requires forall+ (ebid:natlt 1) (etid:natlt 1). f
+  ensures f
+{
+  forevery_singleton_elim #(natlt 1) _;
+  forevery_singleton_elim #(natlt 1) _;
+}
+
+
+inline_for_extraction noextract
+fn kernel_nop (eshmem : erased (gpu_array u32 0sz)) (ebid : enatlt 1sz) (etid : enatlt 1sz)
+  requires
+    gpu **
+    emp ** (* kpre *)
+    thread_id 1sz etid **
+    block_id 1sz ebid **
+    shmem_tok eshmem **
+    emp (* block pre *)
+  ensures
+    gpu **
+    emp ** (* kpost *)
+    thread_id 1sz etid **
+    block_id 1sz ebid **
+    shmem_tok eshmem **
+    emp (* block post *)
+{
+  ()
+}
+
+inline_for_extraction noextract
+let nop_desc : kernel_desc emp emp = {
+  nblk = 1sz;
+  nthr = 1sz;
+
+  shmem_type = u32;
+  shmem_type_is_sized = solve;
+  shmem_sz = 0sz;
+
+  block_pre  = (fun _ _ _ -> emp);
+  block_post = (fun _ _ _ -> emp);
+  block_setup = nop_block_setup;
+
+  kpre = (fun _ _ -> emp);
+  kpost = (fun _ _ -> emp);
+  f = kernel_nop;
+
+  setup = ghost_setup;
+  teardown = ghost_teardown;
+}
+
+inline_for_extraction noextract
+fn kf_no_shmem
+  (#nblk : (x : SZ.t { 0 < x /\ x <= max_blocks }))
+  (#nthr : (x : SZ.t { 0 < x /\ x <= max_threads }))
+  (#shmem_type : Type0)
+  {| shmem_type_is_sized : Kuiper.Sized.sized shmem_type |}
+  (#shmem_sz : SZ.t)
+  (#kpre  : natlt nblk -> natlt nthr -> slprop)
+  (#kpost : natlt nblk -> natlt nthr -> slprop)
+  (kf : (
+    ebid : enatlt nblk ->
+    etid : enatlt nthr ->
+    stt unit
+      (requires
+         gpu **
+         kpre ebid etid **
+         thread_id nthr etid **
+         block_id nblk ebid
+      )
+      (ensures fun _ ->
+         gpu **
+         kpost ebid etid **
+         thread_id nthr etid **
+         block_id nblk ebid)
+  ))
+  (eshmem : erased (gpu_array shmem_type shmem_sz))
+  (ebid : enatlt nblk)
+  (etid : enatlt nthr)
+  requires
+    gpu **
+    kpre ebid etid **
+    thread_id nthr etid **
+    block_id nblk ebid **
+    shmem_tok eshmem **
+    emp
+  ensures
+    gpu **
+    kpost ebid etid **
+    thread_id nthr etid **
+    block_id nblk ebid **
+    shmem_tok eshmem **
+    emp
+{
+  kf ebid etid
+}
