src/lib/kuiper/Kuiper.Sized.fsti
@@ -2,7 +2,35 @@ module Kuiper.Sized
 
 module SZ = FStar.SizeT
 
+module U8  = FStar.UInt8
+module U16 = FStar.UInt16
+module U32 = FStar.UInt32
+module U64 = FStar.UInt64
+
+module I8  = FStar.Int8
+module I16 = FStar.Int16
+module I32 = FStar.Int32
+module I64 = FStar.Int64
+
+module F16 = Kuiper.Float16
+module F32 = Kuiper.Float32
+module F64 = Kuiper.Float64
+
 inline_for_extraction
 class sized (t:Type) = {
   size : SZ.t;
 }
+
+inline_for_extraction instance _ : sized U8.t  = { size = 1sz; }
+inline_for_extraction instance _ : sized U16.t = { size = 2sz; }
+inline_for_extraction instance _ : sized U32.t = { size = 4sz; }
+inline_for_extraction instance _ : sized U64.t = { size = 8sz; }
+
+inline_for_extraction instance _ : sized I8.t  = { size = 1sz; }
+inline_for_extraction instance _ : sized I16.t = { size = 2sz; }
+inline_for_extraction instance _ : sized I32.t = { size = 4sz; }
+inline_for_extraction instance _ : sized I64.t = { size = 8sz; }
+
+inline_for_extraction instance _ : sized F16.t = { size = 2sz; }
+inline_for_extraction instance _ : sized F32.t = { size = 4sz; }
+inline_for_extraction instance _ : sized F64.t = { size = 8sz; }
