src/lib/poly/Kuiper.MatMul.Tiled.fsti
@@ -9,28 +9,28 @@ open Kuiper.MatMulGPU.Type
 open Kuiper.Matrix.Reprs.Type
 open Kuiper.Matrix4 { mlayout4, clayout4 }
 
-inline_for_extraction
-val kernel_fixed_ty
-  (bdim : pos) (* block dim *)
-  (et : Type0) {| scalar et |}
-  (#mrows #mshared #mcols : pos) (* already divided by bdim *)
-  (lA : mlayout4 mrows   mshared bdim bdim)
-  (lB : mlayout4 mshared mcols   bdim bdim)
-  (lC : mlayout4 mrows   mcols   bdim bdim)
-: Type0
+// inline_for_extraction
+// val kernel_fixed_ty
+//   (bdim : pos) (* block dim *)
+//   (et : Type0) {| scalar et |}
+//   (#mrows #mshared #mcols : pos) (* already divided by bdim *)
+//   (lA : mlayout4 mrows   mshared bdim bdim)
+//   (lB : mlayout4 mshared mcols   bdim bdim)
+//   (lC : mlayout4 mrows   mcols   bdim bdim)
+// : Type0
 
-inline_for_extraction noextract
-val kernel_fixed
-  (bdim : szp) (* block dim *)
-  (#et : Type0) {| scalar et |}
-  (#mrows #mshared #mcols : sz) (* already divided by bdim *)
-  (#lA : mlayout4 mrows   mshared bdim bdim)
-  (#lB : mlayout4 mshared mcols   bdim bdim)
-  (#lC : mlayout4 mrows   mcols   bdim bdim)
-  {| clayout4 lA |}
-  {| clayout4 lB |}
-  {| clayout4 lC |}
-: kernel_fixed_ty bdim et lA lB lC
+// inline_for_extraction noextract
+// val kernel_fixed
+//   (bdim : szp) (* block dim *)
+//   (#et : Type0) {| scalar et |}
+//   (#mrows #mshared #mcols : sz) (* already divided by bdim *)
+//   (#lA : mlayout4 mrows   mshared bdim bdim)
+//   (#lB : mlayout4 mshared mcols   bdim bdim)
+//   (#lC : mlayout4 mrows   mcols   bdim bdim)
+//   {| clayout4 lA |}
+//   {| clayout4 lB |}
+//   {| clayout4 lC |}
+// : kernel_fixed_ty bdim et lA lB lC
 
 // inline_for_extraction noextract
 // val matmul_gpu_fixed_wrap
