Makefile
@@ -49,8 +49,10 @@ dist: all
 
 .PHONY: lint
 lint:
+	./FStar/.scripts/remove_all_unused_opens.sh extraction
 	./FStar/.scripts/remove_all_unused_opens.sh src
 	( cd src && git sed 's/ *$$//' )
+	( cd extraction && git sed 's/ *$$//' )
 	( cd src && ../scripts/find-pulse-noix.sh )
 	( cd src && ../scripts/check-attrs.sh )
 
